src/mqtt-packet-parser/src/debug_ffi.c
@@ -1,15 +1,30 @@
 #include <stdio.h>
 #include <stdint.h>
 
-void print_hex(uint8_t i) {
+void print_hex_u8(uint8_t i) {
   printf("%02x", i);
 }
 
-void print_buffer(uint8_t *buffer, uint32_t buffer_size) {
+void print_hex_u16(uint16_t i) {
+  printf("%02x", i);
+}
+
+void print_buffer_u8(uint8_t *buffer, uint32_t buffer_size) {
   printf("[");
   for (int i = 0; i < buffer_size; i++)
   {
     printf("%02x", buffer[i]);
+    if (i != buffer_size - 1)
+      printf(", ");
+  }
+  puts("]");
+}
+
+void print_buffer_u16(uint16_t *buffer, uint32_t buffer_size) {
+  printf("[");
+  for (int i = 0; i < buffer_size; i++)
+  {
+    printf("%04x", buffer[i]);
     if (i != buffer_size - 1)
       printf(", ");
   }
