src/mqtt-packet-parser/src/debug_ffi.fst
@@ -1,16 +1,27 @@
 module Debug_FFI
 
 module U8 = FStar.UInt8
+module U16 = FStar.UInt16
 module U32 = FStar.UInt32
 module B = LowStar.Buffer
 
 open FStar.HyperStack.ST
 
-assume val print_hex (i:U8.t): Stack unit
+assume val print_hex_u8 (i:U8.t): Stack unit
   (requires (fun h -> true))
   (ensures (fun h0 ret h1 -> true))
 
-assume val print_buffer: (buffer: B.buffer U8.t)
+assume val print_hex_u16 (i:U16.t): Stack unit
+(requires (fun h -> true))
+(ensures (fun h0 ret h1 -> true))
+
+assume val print_buffer_u8: (buffer: B.buffer U8.t)
+-> buffer_size: U32.t
+-> Stack unit
+  (requires (fun h -> true))
+  (ensures (fun h0 ret h1 -> true))
+
+assume val print_buffer_u16: (buffer: B.buffer U16.t)
 -> buffer_size: U32.t
 -> Stack unit
   (requires (fun h -> true))
