src/mqtt-packet-parser/src/ffi.fst
@@ -3,19 +3,26 @@ module FFI
 module U8 = FStar.UInt8
 module U32 = FStar.UInt32
 module B = LowStar.Buffer
+module HS = FStar.HyperStack
 
 open FStar.HyperStack.ST
-open Common
+// open Common
 
 open C
 open LowStar.Printf
 
-assume val topic_name_uint8_to_c_string: u8_buffer: B.buffer U8.t -> Stack C.String.t
+let zero_terminated_buffer_u8 (h: HS.mem) (b: B.buffer U8.t) =
+  let s = B.as_seq h b in
+  B.length b > 0 /\
+  B.length b <= FStar.UInt.max_int 32 /\
+  U8.v (Seq.index s (B.length b - 1)) = 0
+
+assume val uint8_to_c_string: u8_buffer: B.buffer U8.t -> Stack C.String.t
   (requires (fun h -> B.live h u8_buffer /\ zero_terminated_buffer_u8 h u8_buffer /\ B.length u8_buffer = 65536))
   (ensures (fun h0 ret h1 -> U32.v (C.String.strlen ret) <= 65535))
 
 assume val payload_uint8_to_c_string:
-  u8_buffer: B.buffer U8.t
+  u8_buffer: B.buffer (B.buffer U8.t)
   -> min_packet_size: U32.t
   -> max_packet_size: U32.t
   -> packet_size:
