src/mqtt-packet-parser/src/test/testValidPackets.fst
@@ -22,11 +22,11 @@ let print x =  C.String.print x
 val print_struct_fixed_header: s:struct_fixed_header -> St unit
 let print_struct_fixed_header s =
     print !$"message_name: "; print s.message_name; new_line ();
-    print !$"message_type: 0x"; UT.print_hex s.message_type; new_line ();
-    print !$"flag: 0x"; UT.print_hex s.flags.flag; new_line ();
-    print !$"dup_flag: 0x"; UT.print_hex s.flags.dup_flag; new_line ();
-    print !$"qos_flag: 0x"; UT.print_hex s.flags.qos_flag; new_line ();
-    print !$"retain_flag: 0x"; UT.print_hex s.flags.retain_flag; new_line ();
+    print !$"message_type: 0x"; UT.print_hex_u8 s.message_type; new_line ();
+    print !$"flag: 0x"; UT.print_hex_u8 s.flags.flag; new_line ();
+    print !$"dup_flag: 0x"; UT.print_hex_u8 s.flags.dup_flag; new_line ();
+    print !$"qos_flag: 0x"; UT.print_hex_u8 s.flags.qos_flag; new_line ();
+    print !$"retain_flag: 0x"; UT.print_hex_u8 s.flags.retain_flag; new_line ();
     print !$"remaining_length: "; print_u32 s.remaining_length; new_line ();
     print !$"error_message: "; print s.error.message; new_line ()
 
